Blanc.lean
@@ -74,6 +74,7 @@ import Blanc.FmintCode
 import Blanc.FlashSpec
 import Blanc.Compiled
 import Blanc.DeploymentCompiled
+import Blanc.DeploymentMessage
 import Blanc.Forward
 import Blanc.Reverts
 import Blanc.RevertPayload
